Strata/Languages/Boogie/StatementSemantics.lean
@@ -25,7 +25,7 @@ instance : HasVal Boogie.Expression where value := Value
 instance : HasFvar Boogie.Expression where
   mkFvar := (.fvar () · none)
   getFvar
-  | .fvar () v _ => some v
+  | .fvar _ v _ => some v
   | _ => none
 
 @[match_pattern]
@@ -48,19 +48,19 @@ abbrev BoogieEval := SemanticEval Expression
 abbrev BoogieStore := SemanticStore Expression
 
 def WellFormedBoogieEvalCong (δ : BoogieEval) : Prop :=
-    (∀ e₁ e₁' σ₀ σ σ₀' σ',
+    (∀ e₁ e₁' σ₀ σ σ₀' σ' m,
       δ σ₀ σ e₁ = δ σ₀' σ' e₁' →
-      (∀ ty, δ σ₀ σ (.abs () ty e₁) = δ σ₀' σ' (.abs () ty e₁')) ∧
+      (∀ ty, δ σ₀ σ (.abs m ty e₁) = δ σ₀' σ' (.abs m ty e₁')) ∧
     -- binary congruence
     (∀ e₂ e₂',
       δ σ₀ σ e₂ = δ σ₀' σ' e₂' →
-      δ σ₀ σ (.app () e₁ e₂) = δ σ₀' σ' (.app () e₁' e₂') ∧
-      δ σ₀ σ (.eq () e₁ e₂) = δ σ₀' σ' (.eq () e₁' e₂') ∧
-      (∀ k ty, δ σ₀ σ (.quant () k ty e₁ e₂) = δ σ₀' σ' (.quant () k ty e₁' e₂')) ∧
+      δ σ₀ σ (.app m e₁ e₂) = δ σ₀' σ' (.app m e₁' e₂') ∧
+      δ σ₀ σ (.eq m e₁ e₂) = δ σ₀' σ' (.eq m e₁' e₂') ∧
+      (∀ k ty, δ σ₀ σ (.quant m k ty e₁ e₂) = δ σ₀' σ' (.quant m k ty e₁' e₂')) ∧
     -- ternary congruence
     (∀ e₃ e₃',
       δ σ₀ σ e₃ = δ σ₀' σ' e₃' →
-      δ σ₀ σ (.ite () e₃ e₁ e₂) = δ σ₀' σ' (.ite () e₃' e₁' e₂')
+      δ σ₀ σ (.ite m e₃ e₁ e₂) = δ σ₀' σ' (.ite m e₃' e₁' e₂')
     ))
     )
 
@@ -161,13 +161,13 @@ def updatedStates
 def WellFormedBoogieEvalTwoState (δ : BoogieEval) (σ₀ σ : BoogieStore) : Prop :=
     open Boogie.OldExpressions in
       (∃ vs vs' σ₁, HavocVars σ₀ vs σ₁ ∧ InitVars σ₁ vs' σ) ∧
-      (∀ vs vs' σ₀ σ₁ σ,
+      (∀ vs vs' σ₀ σ₁ σ m,
         (HavocVars σ₀ vs σ₁ ∧ InitVars σ₁ vs' σ) →
         -- if the variable is modified, then old variable should lookup in the old store
-        ∀ v,
-          (v ∈ vs → ∀ oty ty, δ σ₀ σ (@oldVar () (tyold := oty) v (tyv := ty)) = σ₀ v) ∧
+        ∀ v mOp mVar,
+          (v ∈ vs → ∀ oty ty, δ σ₀ σ (@oldVar m (tyold := oty) mOp mVar v (tyv := ty)) = σ₀ v) ∧
         -- if the variable is not modified, then old variable is identity
-          (¬ v ∈ vs → ∀ oty ty, δ σ₀ σ (@oldVar () (tyold := oty) v (tyv := ty)) = σ v)) ∧
+          (¬ v ∈ vs → ∀ oty ty, δ σ₀ σ (@oldVar m (tyold := oty) mOp mVar v (tyv := ty)) = σ v)) ∧
       -- evaluating on an old complex expression is the same as evlauating on its normal form
       -- TODO: can possibly break this into more sub-components, proving it using congruence and normalization property
       -- Might not be needed if we assume all expressions are normalized
