Strata/Languages/C_Simp/Examples/Trivial.lean
@@ -45,7 +45,8 @@ Errors: #[]
 #eval Strata.C_Simp.TransM.run (Strata.C_Simp.translateProgram (TrivialPgm.commands))
 
 /--
-info: [Strata.Boogie] Type checking succeeded.
+info: POSTCONDITIONSCHECKS: (post, #true)
+[Strata.Boogie] Type checking succeeded.
 
 
 VCs:
