Strata/Transform/CallElimCorrect.lean
@@ -349,33 +349,30 @@ Imperative.WellFormedSemanticEvalVal δ →
   induction e <;> simp [Imperative.HasVarsPure.getVars, Lambda.LExpr.LExpr.getVars] at *
   case const c t | op o ty | bvar b =>
     rw [Hval]; rw [Hval]; constructor; constructor
-  case fvar n ty =>
+  case fvar m n ty =>
     simp [Hwfv]
     simp [updatedState]
     intros Heq
     simp [Heq]
     simp_all
-  case mdata info e ih =>
-    apply ((Hwfc e e σ₀ (updatedState σ k v) σ₀ σ) ?_).2.1
+  case abs m ty e ih =>
+    apply ((Hwfc e e σ₀ (updatedState σ k v) σ₀ σ) m ?_).1
     apply ih ; simp_all
-  case abs ty e ih =>
-    apply ((Hwfc e e σ₀ (updatedState σ k v) σ₀ σ) ?_).1
-    apply ih ; simp_all
-  case quant kk ty tr e trih eih =>
-    apply (((Hwfc tr tr σ₀ (updatedState σ k v) σ₀ σ) ?_).2.2 e e ?_).2.2.1
+  case quant m kk ty tr e trih eih =>
+    apply ((Hwfc tr tr σ₀ (updatedState σ k v) σ₀ σ m ?_).2 e e ?_).2.2.1
     apply trih ; simp_all
     apply eih ; simp_all
-  case app fn e fnih eih =>
-    apply (((Hwfc fn fn σ₀ (updatedState σ k v) σ₀ σ) ?_).2.2 e e ?_).1
+  case app m fn e fnih eih =>
+    apply (((Hwfc fn fn σ₀ (updatedState σ k v) σ₀ σ) m ?_).2 e e ?_).1
     apply fnih ; simp_all
     apply eih ; simp_all
-  case ite c t e cih tih eih =>
-    apply (((Hwfc t t σ₀ (updatedState σ k v) σ₀ σ) ?_).2.2 e e ?_).2.2.2 c c ?_
+  case ite m c t e cih tih eih =>
+    apply (((Hwfc t t σ₀ (updatedState σ k v) σ₀ σ) m ?_).2 e e ?_).2.2.2 c c ?_
     apply tih ; simp_all
     apply eih ; simp_all
     apply cih ; simp_all
-  case eq e1 e2 e1ih e2ih =>
-    apply (((Hwfc e1 e1 σ₀ (updatedState σ k v) σ₀ σ) ?_).2.2 e2 e2 ?_).2.1
+  case eq m e1 e2 e1ih e2ih =>
+    apply (((Hwfc e1 e1 σ₀ (updatedState σ k v) σ₀ σ) m ?_).2 e2 e2 ?_).2.1
     apply e1ih ; simp_all
     apply e2ih ; simp_all
 
@@ -632,7 +629,7 @@ theorem EvalStatementContractInitVar :
   constructor
   constructor
   . apply Imperative.EvalCmd.eval_init <;> try assumption
-    have Hwfv := Hwf (Lambda.LExpr.fvar v none) v σ₀ σ
+    have Hwfv := Hwf (Lambda.LExpr.fvar () v none) v σ₀ σ
     rw [Hwfv]; assumption
     simp [Imperative.HasFvar.getFvar]
     apply Imperative.InitState.init Hnone
@@ -1160,19 +1157,13 @@ theorem Lambda.LExpr.substFvarCorrect :
       exact Hinv
       simp [Imperative.HasFvar.getFvar]
       simp [Imperative.HasFvar.getFvar]
-  case mdata info e ih =>
+  case abs m ty e ih  =>
     simp [Boogie.WellFormedBoogieEvalCong] at Hwfc
     specialize ih Hinv
-    specialize Hwfc _ _ _ _ _ _ ih
-    have Hinfo := Hwfc.2.1
-    specialize Hinfo info
-    simp [Hinfo]
-  case abs ty e ih  =>
-    simp [Boogie.WellFormedBoogieEvalCong] at Hwfc
-    specialize ih Hinv
-    specialize Hwfc _ _ _ _ _ _ ih
-    apply Hwfc.1
-  case quant k ty tr e trih eih =>
+    have e2 := (e.substFvar fro (Lambda.LExpr.fvar () to none))
+    have Hwfcx := Hwfc e ((e.substFvar fro (Lambda.LExpr.fvar () to none))) σ₀ σ σ₀' σ' m ih |>.1
+    apply Hwfcx
+  case quant m k ty tr e trih eih =>
     simp [Boogie.WellFormedBoogieEvalCong] at Hwfc
     simp [Imperative.invStores, Imperative.substStores,
           Imperative.HasVarsPure.getVars, Lambda.LExpr.LExpr.getVars] at *
@@ -1187,12 +1178,12 @@ theorem Lambda.LExpr.substFvarCorrect :
       rw [Hinv]
       left;
       assumption
-    specialize Hwfc _ _ _ _ _ _ trih
-    have Hfun := Hwfc.2.2
+    have Hwfc := Hwfc tr (tr.substFvar fro (Lambda.LExpr.fvar () to none)) σ₀ σ σ₀' σ' m trih
+    have Hfun := Hwfc.2
     specialize Hfun _ _ eih
     have Hfun := Hfun.2.2.1
     exact (Hfun k ty)
-  case app c fn fih eih =>
+  case app m c fn fih eih =>
     simp [Boogie.WellFormedBoogieEvalCong] at Hwfc
     simp [Imperative.invStores, Imperative.substStores,
           Imperative.HasVarsPure.getVars, Lambda.LExpr.LExpr.getVars] at *
@@ -1205,12 +1196,12 @@ theorem Lambda.LExpr.substFvarCorrect :
     . intros k1 k2 Hin
       rw [Hinv]
       right; assumption
-    specialize Hwfc _ _ _ _ _ _ fih
-    have Hfun := Hwfc.2.2
+    have Hwfc := Hwfc c (c.substFvar fro (Lambda.LExpr.fvar () to none)) σ₀ σ σ₀' σ' m fih
+    have Hfun := Hwfc.2
     specialize Hfun _ _ eih
     have Hfun := Hfun.1
     exact Hfun
-  case ite c t e cih tih eih =>
+  case ite m c t e cih tih eih =>
     simp [Boogie.WellFormedBoogieEvalCong] at Hwfc
     simp [Imperative.invStores, Imperative.substStores,
           Imperative.HasVarsPure.getVars, Lambda.LExpr.LExpr.getVars] at *
@@ -1227,13 +1218,13 @@ theorem Lambda.LExpr.substFvarCorrect :
     . intros k1 k2 Hin
       rw [Hinv]
       right; right; assumption
-    specialize Hwfc _ _ _ _ _ _ tih
-    have Hfun := Hwfc.2.2
+    have Hwfc := Hwfc t (t.substFvar fro (Lambda.LExpr.fvar () to none)) σ₀ σ σ₀' σ' m tih
+    have Hfun := Hwfc.2
     specialize Hfun _ _ eih
     have Hfun := Hfun.2.2.2
     specialize Hfun _ _ cih
     exact Hfun
-  case eq e1 e2 e1ih e2ih =>
+  case eq m e1 e2 e1ih e2ih =>
     simp [Boogie.WellFormedBoogieEvalCong] at Hwfc
     simp [Imperative.invStores, Imperative.substStores,
           Imperative.HasVarsPure.getVars, Lambda.LExpr.LExpr.getVars] at *
@@ -1246,8 +1237,8 @@ theorem Lambda.LExpr.substFvarCorrect :
     . intros k1 k2 Hin
       rw [Hinv]
       right; assumption
-    specialize Hwfc _ _ _ _ _ _ e1ih
-    have Hfun := Hwfc.2.2
+    specialize Hwfc e1 (e1.substFvar fro (Lambda.LExpr.fvar () to none)) σ₀ σ σ₀' σ' m e1ih
+    have Hfun := Hwfc.2
     specialize Hfun _ _ e2ih
     have Hfun := Hfun.2.1
     exact Hfun
@@ -1265,28 +1256,21 @@ theorem Lambda.LExpr.substFvarsCorrectZero :
     rw [Hwfvl.2]
     constructor
     constructor
-  case fvar name ty =>
+  case fvar m name ty =>
     simp [Imperative.WellFormedSemanticEvalVar] at Hwfvr
-    specialize Hwfvr (Lambda.LExpr.fvar name ty) name
+    specialize Hwfvr (Lambda.LExpr.fvar m name ty) name
     rw [Hwfvr]
     rw [Hwfvr]
     rw [Hinv]
     simp [Imperative.HasVarsPure.getVars, Lambda.LExpr.LExpr.getVars]
     simp [Imperative.HasFvar.getFvar]
     simp [Imperative.HasFvar.getFvar]
-  case mdata info e ih =>
+  case abs m ty e ih  =>
     simp [Boogie.WellFormedBoogieEvalCong] at Hwfc
     specialize ih Hinv
-    specialize Hwfc _ _ _ _ _ _ ih
-    have Hinfo := Hwfc.2.1
-    specialize Hinfo info
-    simp [Hinfo]
-  case abs ty e ih  =>
-    simp [Boogie.WellFormedBoogieEvalCong] at Hwfc
-    specialize ih Hinv
-    specialize Hwfc _ _ _ _ _ _ ih
+    have Hwfc := Hwfc e e σ₀ σ σ₀' σ' m ih
     apply Hwfc.1
-  case quant k ty tr e trih eih =>
+  case quant m k ty tr e trih eih =>
     simp [Boogie.WellFormedBoogieEvalCong] at Hwfc
     simp [Imperative.invStores, Imperative.substStores,
           Imperative.HasVarsPure.getVars, Lambda.LExpr.LExpr.getVars] at *
@@ -1299,12 +1283,12 @@ theorem Lambda.LExpr.substFvarsCorrectZero :
     . intros k1 k2 Hin
       rw [Hinv]
       right; assumption
-    specialize Hwfc _ _ _ _ _ _ trih
-    have Hfun := Hwfc.2.2
+    have Hwfc := Hwfc tr tr σ₀ σ σ₀' σ' m trih
+    have Hfun := Hwfc.2
     specialize Hfun _ _ eih
     have Hfun := Hfun.2.2.1
     exact (Hfun k ty)
-  case app c fn fih eih =>
+  case app m fn e fih eih =>
     simp [Boogie.WellFormedBoogieEvalCong] at Hwfc
     simp [Imperative.invStores, Imperative.substStores,
           Imperative.HasVarsPure.getVars, Lambda.LExpr.LExpr.getVars] at *
@@ -1317,12 +1301,12 @@ theorem Lambda.LExpr.substFvarsCorrectZero :
     . intros k1 k2 Hin
       rw [Hinv]
       right; assumption
-    specialize Hwfc _ _ _ _ _ _ fih
-    have Hfun := Hwfc.2.2
+    have Hwfc := Hwfc fn fn σ₀ σ σ₀' σ' m fih
+    have Hfun := Hwfc.2
     specialize Hfun _ _ eih
     have Hfun := Hfun.1
     exact Hfun
-  case ite c t e cih tih eih =>
+  case ite m c t e cih tih eih =>
     simp [Boogie.WellFormedBoogieEvalCong] at Hwfc
     simp [Imperative.invStores, Imperative.substStores,
           Imperative.HasVarsPure.getVars, Lambda.LExpr.LExpr.getVars] at *
@@ -1339,13 +1323,13 @@ theorem Lambda.LExpr.substFvarsCorrectZero :
     . intros k1 k2 Hin
       rw [Hinv]
       right; right; assumption
-    specialize Hwfc _ _ _ _ _ _ tih
-    have Hfun := Hwfc.2.2
+    have Hwfc := Hwfc t t  σ₀ σ σ₀' σ' m tih
+    have Hfun := Hwfc.2
     specialize Hfun _ _ eih
     have Hfun := Hfun.2.2.2
     specialize Hfun _ _ cih
     exact Hfun
-  case eq e1 e2 e1ih e2ih =>
+  case eq m e1 e2 e1ih e2ih =>
     simp [Boogie.WellFormedBoogieEvalCong] at Hwfc
     simp [Imperative.invStores, Imperative.substStores,
           Imperative.HasVarsPure.getVars, Lambda.LExpr.LExpr.getVars] at *
@@ -1358,8 +1342,8 @@ theorem Lambda.LExpr.substFvarsCorrectZero :
     . intros k1 k2 Hin
       rw [Hinv]
       right; assumption
-    specialize Hwfc _ _ _ _ _ _ e1ih
-    have Hfun := Hwfc.2.2
+    have Hwfc := Hwfc e1 e1 σ₀ σ σ₀' σ' m e1ih
+    have Hfun := Hwfc.2
     specialize Hfun _ _ e2ih
     have Hfun := Hfun.2.1
     exact Hfun
@@ -1809,24 +1793,15 @@ theorem substOldCorrect :
     exact name
     simp [Imperative.HasFvar.getFvar]
     simp [Imperative.HasFvar.getFvar]
-  case mdata info e ih =>
-    simp [Boogie.WellFormedBoogieEvalCong] at Hwfc
-    cases Hnorm with
-    | mdata Hnorm =>
-    specialize ih Hnorm Hinv
-    specialize Hwfc _ _ _ _ _ _ ih
-    have Hinfo := Hwfc.2.1
-    specialize Hinfo info
-    simp [Hinfo]
-  case abs ty e ih  =>
+  case abs m ty e ih  =>
     simp [Boogie.WellFormedBoogieEvalCong] at Hwfc
     cases Hnorm with
     | abs Hnorm =>
     specialize ih Hnorm
     specialize ih Hinv
-    specialize Hwfc _ _ _ _ _ _ ih
+    have Hwfc := Hwfc e (OldExpressions.substOld fro (createFvar to) e) σ₀ σ σ₀' σ m ih
     apply Hwfc.1
-  case quant k ty tr e trih eih =>
+  case quant m k ty tr e trih eih =>
     simp [Boogie.WellFormedBoogieEvalCong] at Hwfc
     cases Hnorm with
     | quant Ht He =>
@@ -1844,12 +1819,12 @@ theorem substOldCorrect :
             List.app_removeAll,
             List.zip_append]
       right; assumption
-    specialize Hwfc _ _ _ _ _ _ trih
-    have Hfun := Hwfc.2.2
+    have Hwfc := Hwfc tr (OldExpressions.substOld fro (createFvar to) tr) σ₀ σ σ₀' σ m trih
+    have Hfun := Hwfc.2
     specialize Hfun _ _ eih
     have Hfun := Hfun.2.2.1
     exact (Hfun k ty)
-  case app c fn fih eih =>
+  case app m c fn fih eih =>
     cases Hnorm with
     | app Hc Hfn Hwf =>
     specialize fih Hc ?_
@@ -1890,9 +1865,9 @@ theorem substOldCorrect :
         cases Hwf2' with
         | intro σ₁ Hwf2' =>
         by_cases Hin : fro ∈ vs
-        case pos e1 e2 ty' =>
+        case pos =>
         -- old var is modified
-          have HH := ((Hwf2.2.1 vs vs' σ₀ σ₁ σ Hwf2'.1 Hwf2'.2) fro).1 Hin
+          have HH := fun m2 mOp mVar => Hwf2.2.1 vs vs' σ₀ σ₁ σ m2 Hwf2'.1 Hwf2'.2 fro mOp mVar |>.1 Hin
           simp [OldExpressions.oldVar,
                 OldExpressions.oldExpr,
                 BoogieIdent.unres] at HH
@@ -1903,7 +1878,7 @@ theorem substOldCorrect :
           apply Hsubst
           exact List.mem_singleton.mpr rfl
           simp [Imperative.HasFvar.getFvar]
-        case neg e1 e2 ty' =>
+        case neg =>
         -- old var is not modified
           have Hup := HavocVarsUpdateStates Hwf2'.1
           cases Hup with
@@ -1913,7 +1888,7 @@ theorem substOldCorrect :
           | intro bs Hinit =>
           have Hsubst' := substStoresUpdatesInv' ?_ Hsubst Hup
           have Hsubst'' := substStoresInitsInv' ?_ Hsubst' Hinit
-          . have HH := ((Hwf2.2.1 _ _ _ _ _ Hwf2'.1 Hwf2'.2) fro).2 Hin
+          . have HH := fun m2 mOp mVar => Hwf2.2.1 _ _ _ _ _ m2 Hwf2'.1 Hwf2'.2 fro mOp mVar |>.2 Hin
             simp [OldExpressions.oldVar,
                   OldExpressions.oldExpr,
                   BoogieIdent.unres] at HH
@@ -1936,18 +1911,27 @@ theorem substOldCorrect :
             simp [Heq] at *
             contradiction
       . -- is an old var that is not substituted, use congruence
-        specialize Hwfc _ _ _ _ _ _ fih
-        have Hfun := Hwfc.2.2
-        specialize Hfun _ _ eih
-        have Hfun := Hfun.1
-        exact Hfun
+        rename_i e1 e2 mOp ty0 mVar x ty1 h
+        simp at m mOp ty0 mVar x ty1
+        unfold WellFormedBoogieEvalCong at Hwfc
+        let eHelper: Expression.Expr := Lambda.LExpr.op m (Visibility.unres, "old") ty0
+        let eHelper2: Expression.Expr := Lambda.LExpr.fvar mVar x ty1
+        have Hwfc2 := Hwfc eHelper eHelper σ₀ σ σ₀' σ m
+        rw [OldExpressions.substOld] at fih
+        unfold createFvar at eih
+        rw [OldExpressions.substOld] at eih
+        have Hwfc3 := Hwfc2 fih |>.2 eHelper2 eHelper2
+        have Hwfc4 := Hwfc3 eih |>.1
+        assumption
     . -- is not an old var, use congruence
-      specialize Hwfc _ _ _ _ _ _ fih
-      have Hfun := Hwfc.2.2
+      unfold WellFormedBoogieEvalCong at Hwfc
+      let eHelper2: Expression.Expr := (OldExpressions.substOld fro (createFvar to) c)
+      have Hwfc2 := Hwfc c eHelper2 σ₀ σ σ₀' σ m fih
+      have Hfun := Hwfc2.2
       specialize Hfun _ _ eih
       have Hfun := Hfun.1
       exact Hfun
-  case ite c t e cih tih eih =>
+  case ite m c t e cih tih eih =>
     simp [Boogie.WellFormedBoogieEvalCong] at Hwfc
     cases Hnorm with
     | ite Hc Ht He =>
@@ -1972,13 +1956,16 @@ theorem substOldCorrect :
             List.app_removeAll,
             List.zip_append]
       right; right; assumption
-    specialize Hwfc _ _ _ _ _ _ tih
-    have Hfun := Hwfc.2.2
-    specialize Hfun _ _ eih
+    let tExpr: Expression.Expr := (OldExpressions.substOld fro (createFvar to) t)
+    let eExpr: Expression.Expr := (OldExpressions.substOld fro (createFvar to) e)
+    --have Hwfc2 := HWfc t tExpr
+    specialize Hwfc t tExpr σ₀ σ σ₀' σ m tih
+    have Hfun := Hwfc.2 e eExpr
+    specialize Hfun eih
     have Hfun := Hfun.2.2.2
     specialize Hfun _ _ cih
     exact Hfun
-  case eq e1 e2 e1ih e2ih =>
+  case eq m e1 e2 e1ih e2ih =>
     simp [Boogie.WellFormedBoogieEvalCong] at Hwfc
     cases Hnorm with
     | eq He1 He2 =>
@@ -1996,8 +1983,10 @@ theorem substOldCorrect :
             List.app_removeAll,
             List.zip_append]
       right; assumption
-    specialize Hwfc _ _ _ _ _ _ e1ih
-    have Hfun := Hwfc.2.2
+    let e1Expr: Expression.Expr := (OldExpressions.substOld fro (createFvar to) e1)
+    let e2Expr: Expression.Expr := (OldExpressions.substOld fro (createFvar to) e2)
+    specialize Hwfc e1 e1Expr σ₀ σ σ₀' σ m e1ih
+    have Hfun := Hwfc.2
     specialize Hfun _ _ e2ih
     have Hfun := Hfun.2.1
     exact Hfun
@@ -2191,7 +2180,7 @@ NormalizedOldExpr e →
 (extractOldExprVars e).removeAll [h] := by
   intros Hnorm
   induction Hnorm <;> simp [extractOldExprVars, createFvar, substOld] at * <;> try assumption
-  case app fn e Hnfn Hne Hwf ih1 ih2 =>
+  case app fn e m Hnfn Hne Hwf ih1 ih2 =>
     split
     . -- is old var
       next e1 e2 ty x ty =>
@@ -2205,7 +2194,10 @@ NormalizedOldExpr e →
         cases Hwf
         simp_all
         simp [BoogieIdent.unres] at HH
-      have Hnold' : ¬ IsOldPred (substOld h (Lambda.LExpr.fvar h' none) fn) := by
+        rename_i md tyy id v
+        have HH2 := HH md tyy () id v
+        simp_all
+      have Hnold' : ¬ IsOldPred (substOld h (Lambda.LExpr.fvar () h' none) fn) := by
         intros Hold
         apply Hnold
         apply substOldIsOldPred' ?_ Hold
@@ -2218,7 +2210,13 @@ NormalizedOldExpr e →
         exfalso; apply Hnold'; constructor
       . -- old expr, contradiction
         exfalso; apply Hnold'; constructor
-      split <;> simp_all
+      split
+      · rename_i x1 x2 x3 m1 id ty2 x7
+        have hI: Lambda.LExpr.op x2 (Visibility.unres, "old") x3 = Lambda.LExpr.op x2 (Visibility.unres, "old") x3 := by rfl
+        have hI2: Lambda.LExpr.fvar m1 id ty2 = Lambda.LExpr.fvar m1 id ty2 := by rfl
+        have h2 := HH x2 x3 m1 id ty2 hI hI2
+        exfalso
+        contradiction
       . -- old expr, contradiction
         exfalso; apply Hnold; constructor
       . simp [List.app_removeAll]
@@ -3019,7 +3017,7 @@ theorem extractedOldExprInVars :
         exact H2
         intros x Hin
         simp_all
-  case mdata ih | abs ih =>
+  case abs ih =>
     cases Hnorm
     apply ih <;> assumption
   case quant trih eih =>
@@ -3215,12 +3213,36 @@ theorem extractedOldVarsInVars :
 open OldExpressions in
 theorem substOldPostSubset:
   (Imperative.HasVarsPure.getVars (P:=Expression)
-    (substOld h2 (Lambda.LExpr.fvar h1 ty) post)).Subset
+    (substOld h2 (Lambda.LExpr.fvar m h1 ty) post)).Subset
     (Imperative.HasVarsPure.getVars (P:=Expression) post ++ [h1]) := by
   induction post <;> simp [substOld]
-  case fvar | op | const | bvar =>
-    intros x Hin ; simp_all
-  case mdata ih | abs ih =>
+  case fvar =>
+    intros x Hin
+    rename_i m name ty2
+    simp at m
+    simp at name
+    simp at ty2
+
+    simp_all
+  case op =>
+    intros x Hin
+    rename_i m name ty2
+    simp at m
+    simp at name
+    simp at ty2
+    simp_all
+  case const =>
+    intros x Hin
+    rename_i m name ty2
+    simp at m
+    simp at ty2
+    simp_all
+  case bvar =>
+    intros x Hin
+    rename_i m d
+    simp at m
+    simp_all
+  case abs ih =>
     exact ih
   case ite cih tih eih =>
     simp [Imperative.HasVarsPure.getVars, Lambda.LExpr.LExpr.getVars] at *
@@ -3266,6 +3288,8 @@ theorem substOldPostSubset:
     . apply List.Subset.trans
       apply trih <;> assumption
       intros x Hin
+      rename_i m1 k1 ty1 trigger1 e1
+      have assoc := List.append_assoc (Lambda.LExpr.LExpr.getVars trigger1) (Lambda.LExpr.LExpr.getVars e1) [h1]
       simp_all
       cases Hin <;> simp_all
     . apply List.Subset.trans
@@ -3300,7 +3324,7 @@ theorem substsOldPostSubset:
   case cons h t ih =>
     apply List.Subset.trans
       (b:=(Imperative.HasVarsPure.getVars
-            (P:=Expression) (substOld h.snd (Lambda.LExpr.fvar h.1.fst none) post)) ++
+            (P:=Expression) (substOld h.snd (Lambda.LExpr.fvar () h.1.fst none) post)) ++
             List.map (Prod.fst ∘ Prod.fst) t)
     . -- apply ih
       -- intros x Hin1 Hin2
@@ -3317,7 +3341,7 @@ theorem substsOldPostSubset:
 
 set_option maxHeartbeats 500000
 -- Second, the program/statement returned by callElim has the same semantics as the pre-transformation program/statement
-theorem callElimStatementCorrect :
+theorem callElimStatementCorrect [LawfulBEq Expression.Expr] :
   -- procedure lookup function is well-behaved
   (∀ pname, π pname = (Program.Procedure.find? p (.unres pname))) →
   -- all global variables in p exist in σ
@@ -4371,8 +4395,8 @@ theorem callElimStatementCorrect :
                                     exact UpdateStatesNotDefMonotone' Hndef Hupdate
                               . exact (List.nodup_append.mp Hgennd).2.1
                               . simp [Houttriplen]
-                          . intros vs vs' σ₀ σ₁ σ Hhav Hinit
-                            have HH := Hwf2.1 vs vs' σ₀ σ₁ σ ⟨Hhav,Hinit⟩
+                          . intros vs vs' σ₀ σ₁ σ m Hhav Hinit
+                            have HH := Hwf2.1 vs vs' σ₀ σ₁ σ m ⟨Hhav,Hinit⟩
                             apply HH
                         -- normalized
                         . apply OldExpressions.normalizeOldExprSound
